Change jellyfish code and proofs to be more consistent with paper

jellyfish/code.v
@@ -18,162 +18,111 @@ Module SkipList (Params: SKIP_LIST_PARAMS).
   
   Definition tail : node_rep := (INT_MAX, dummy_null, dummy_null, None, dummy_lock, dummy_null).
 
-  (* Skip list constructor *)  
   Definition initLocks : val := 
-    rec: "locks" "pt" "lvl" :=
-      if: "lvl" = #(MAX_HEIGHT + 1)
-      then #()
-      else 
-        "pt" +ₗ "lvl" <- newlock #();;
-        "locks" "pt" ("lvl" + #1).
+    rec: "init" "locks" "lvl" :=
+      if: "lvl" = #(MAX_HEIGHT + 1) then #()
+      else "locks" +ₗ "lvl" <- newlock #();;
+           "init" "locks" ("lvl" + #1).
 
   Definition new : val := 
     λ: "_", 
-      let: "np" := ref (rep_to_node tail) in
-      let: "next" := AllocN #(MAX_HEIGHT + 1) "np" in
+      let: "next" := AllocN #(MAX_HEIGHT + 1) (ref (rep_to_node tail)) in
       let: "locks" := AllocN #(MAX_HEIGHT + 1) #() in
         initLocks "locks" #0;;
         ref (#INT_MIN, #dummy_null, "next", NONEV, dummy_lock, "locks").
 
-  (* Find function *)
   Definition find : val := 
     rec: "find" "pred" "k" "lvl" :=
-      let: "np" := nodeNext "pred" in
-      let: "succ" := ! !("np" +ₗ "lvl") in
-      let: "ck" := nodeKey "succ" in
-        if: "k" ≤ "ck"
-        then ("pred", "succ")
+      let: "succ" := ! !(nodeNext "pred" +ₗ "lvl") in
+        if: "k" ≤ nodeKey "succ" then ("pred", "succ")
         else "find" "succ" "k" "lvl".
   
   Definition findLock : val := 
-    rec: "find" "head" "k" "lvl" :=
-      let: "pair" := find "head" "k" "lvl" in
-      let: "pred" := Fst "pair" in
-      let: "curr" := Snd "pair" in
-      let: "locks" := nodeLocks "pred" in
-      let: "lock" := !("locks" +ₗ "lvl") in
-        acquire "lock";;
-        let: "np" := nodeNext "pred" in
-        let: "next" := ! !("np" +ₗ "lvl") in
-        let: "nk" := nodeKey "next" in
-        let: "ck" := nodeKey "curr" in
-          if: "nk" = "ck" 
-          then "pair"
-          else
-            release "lock";;
-            "find" "pred" "k" "lvl".
-
-  (* Skip list lookup *)
-  Definition findPred : val := 
-    rec: "find" "pred" "k" "lvl" := 
+    rec: "find" "pred" "k" "lvl" :=
       let: "pair" := find "pred" "k" "lvl" in
-        if: "lvl" = #0
-        then "pair"
-        else 
-          let: "pred" := Fst "pair" in
-            "find" "pred" "k" ("lvl" - #1).
+      let: "pred" := Fst "pair" in
+      let: "lock" := !(nodeLocks "pred" +ₗ "lvl") in
+        acquire "lock";;
+        let: "succ" := ! !(nodeNext "pred" +ₗ "lvl") in
+          if: "k" ≤ nodeKey "succ" then ("pred", "succ")
+          else release "lock";;
+               "find" "succ" "k" "lvl".
+
+  Definition findAll : val := 
+    rec: "find" "pred" "k" "lvl" "h" := 
+      let: "pair" := find "pred" "k" "lvl" in
+      let: "pred" := Fst "pair" in
+        if: "lvl" = "h" then "pair"
+        else "find" "pred" "k" ("lvl" - #1) "h".
 
   Definition get : val :=
-    λ: "head" "k", 
-      let: "np" := !"head" in
-      let: "pair" := findPred "np" "k" #MAX_HEIGHT in
-      let: "curr" := Snd "pair" in
-      let: "ck" := nodeKey "curr" in
-        if: "k" = "ck"
-        then 
-          let: "val" := nodeVal "curr" in
-            SOME (Fst !"val")
-        else NONEV.
+    λ: "p" "k", 
+      let: "pair" := findAll !"p" "k" #MAX_HEIGHT #0 in
+      let: "succ" := Snd "pair" in
+        if: "k" ≠ nodeKey "succ" then NONEV
+        else let: "val" := !(nodeVal "succ") in SOME (Fst "val").
 
-  (* Link node in lazy list *)
+  Definition link : val := 
+    λ: "pred" "lvl" "n",
+      let: "new" := !"n" in
+        nodeNext "new" +ₗ "lvl" <- !(nodeNext "pred" +ₗ "lvl") ;;
+        nodeLocks "new" +ₗ "lvl" <- newlock #();;
+        nodeNext "pred" +ₗ "lvl" <- "n".
+
+  Definition insert : val := 
+    λ: "pred" "lvl" "n",
+      let: "k" := nodeKey !"n" in
+      let: "pair" := findLock "pred" "k" "lvl" in
+      let: "pred" := Fst "pair" in
+      let: "lock" := !(nodeLocks "pred" +ₗ "lvl") in
+        link "pred" "lvl" "n";;
+        release "lock".
+
   Definition createAndLink : val := 
     λ: "pred" "k" "v" "t" "h",
-      let: "np" := nodeNext "pred" in
-      let: "succ" := !"np" in
       let: "next" := AllocN ("h" + #1) #() in
       let: "locks" := AllocN ("h" + #1) #() in
       let: "val" := ref ("v", "t", #dummy_null) in
-      let: "node" := ref ("k", "val", "next", NONEV, #(), "locks") in
-        "next" <- "succ";;
-        "locks" <- newlock #();;
-        "np" <- "node";;
-        "node".
+      let: "n" := ref ("k", "val", "next", NONEV, #(), "locks") in
+        link "pred" #0 "n";;
+        "n".
 
-  Definition link : val := 
-    λ: "pred" "lvl" "node",
-      let: "np" := nodeNext "pred" in
-      let: "succ" := !("np" +ₗ "lvl") in
-      let: "next" := nodeNext !"node" in
-      let: "locks" := nodeLocks !"node" in
-        ("next" +ₗ "lvl") <- "succ";;
-        ("locks" +ₗ "lvl") <- newlock #();;
-        ("np" +ₗ "lvl") <- "node".
-
-  (* Lazy list insertion *)
   Definition update : val := 
-    λ: "curr" "v" "t",
-      let: "vp" := nodeVal "curr" in
-      let: "val" := !"vp" in
-      let: "ts" := valTs "val" in
-        if: "t" < "ts" 
-        then #()
-        else "vp" <- ("v", "t", ref "val").
+    λ: "node" "v" "t",
+      let: "val" := !(nodeVal "node") in
+        if: "t" < valTs "val" then #()
+        else nodeVal "node" <- ("v", "t", ref "val").
 
   Definition tryInsert : val := 
-    λ: "head" "k" "v" "t" "h",
-      let: "pair" := findLock "head" "k" #0 in
+    λ: "pred" "k" "v" "t" "h",
+      let: "pair" := findLock "pred" "k" #0 in
       let: "pred" := Fst "pair" in
+      let: "succ" := Snd "pair" in
       let: "lock" := !(nodeLocks "pred") in
-      let: "curr" := Snd "pair" in
-      let: "ck" := nodeKey "curr" in
-        if: "k" = "ck"
-        then 
-          update "curr" "v" "t";;
-          release "lock";;
-          NONEV
-        else 
-          let: "node" := createAndLink "pred" "k" "v" "t" "h" in
-            release "lock";;
-            SOME "node".
-
-  Definition insert : val := 
-    λ: "head" "lvl" "node",
-      let: "k" := nodeKey !"node" in
-      let: "pair" := findLock "head" "k" "lvl" in
-      let: "pred" := Fst "pair" in
-      let: "lock" := !(nodeLocks "pred" +ₗ "lvl") in
-        link "pred" "lvl" "node";;
-        release ("lock").
-
-  (* Skip list insertion *)
-  Definition topLevel : val := 
-    rec: "loop" "head" "k" "h" "lvl" :=
-      let: "pair" := find "head" "k" "lvl" in
-      let: "pred" := Fst "pair" in
-        if: "h" = "lvl"
-        then "pred"
-        else "loop" "pred" "k" "h" ("lvl" - #1).
+        if: "k" = nodeKey "succ"
+        then update "succ" "v" "t";;
+             release "lock";;
+             NONEV
+        else let: "n" := createAndLink "pred" "k" "v" "t" "h" in
+               release "lock";;
+               SOME "n".
       
-  Definition putAll : val := 
-    rec: "put" "head" "k" "v" "t" "h" "lvl" := 
-      let: "pair" := find "head" "k" "lvl" in
-      let: "pred" := Fst "pair" in
-        if: "lvl" = #0
-        then tryInsert "pred" "k" "v" "t" "h"
-        else
-          let: "onode" := "put" "pred" "k" "v" "t" "h" ("lvl" - #1) in
-            match: "onode" with
-              NONE => NONEV
-            | SOME "node" =>
-              insert "pred" "lvl" "node";;
-              SOME "node"
-            end.
+  Definition insertAll : val := 
+    rec: "insert" "curr" "k" "v" "t" "h" "lvl" := 
+      if: "lvl" = #0 then tryInsert "curr" "k" "v" "t" "h"
+      else let: "pair" := find "curr" "k" ("lvl" - #1) in
+           let: "pred" := Fst "pair" in
+           let: "opt" := "insert" "pred" "k" "v" "t" "h" ("lvl" - #1) in
+             match: "opt" with
+               NONE => NONEV
+             | SOME "n" => insert "curr" "lvl" "n";;
+                           SOME "n"
+             end.
 
   Definition put : val := 
-    λ: "head" "k" "v" "t" "h",
-      let: "np" := !"head" in
-      let: "pred" := topLevel "np" "k" "h" #MAX_HEIGHT in
-      let: "_" := putAll "pred" "k" "v" "t" "h" "h" in
-        #().
+    λ: "p" "k" "v" "t" "h",
+      let: "pair" := findAll !"p" "k" #MAX_HEIGHT "h" in
+      let: "pred" := Fst "pair" in
+      let: "_" := insertAll "pred" "k" "v" "t" "h" "h" in #().
 
 End SkipList.
