jellyfish/inv/skip_inv.v
@@ -17,7 +17,7 @@ Module SkipListInv (Params: SKIP_LIST_PARAMS).
   Section Proofs.
     Context `{!heapGS Σ, !skipGS Σ, !lockG Σ}.
 
-    Fixpoint skip_list_equiv (lvl: Z) (head: node_rep) (Smap: gmap Z (argmax Z)) 
+    Fixpoint skip_list_equiv (lvl: Z) (head: node_rep) (M: gmap Z (argmax Z)) 
       (q: frac) (bot: bot_gname) (subs: list sub_gname) : iProp Σ :=
       match subs with
       | nil => False
@@ -26,55 +26,53 @@ Module SkipListInv (Params: SKIP_LIST_PARAMS).
         | nil =>
           ⌜ lvl = 0 ⌝
           ∗
-          is_bot_list lvl head Smap q bot top_sub
+          is_bot_list 0 head M q bot top_sub
 
         | bot_sub :: _ =>
           ⌜ lvl > 0 ⌝
           ∗
           is_sub_list lvl head bot top_sub bot_sub
           ∗
-          skip_list_equiv (lvl - 1) head Smap q bot bot_subs
+          skip_list_equiv (lvl - 1) head M q bot bot_subs
         end
       end.
 
-    Definition is_skip_list (v: val) (Smap: gmap Z (argmax Z)) (q: frac) 
+    Definition is_skip_list (p: loc) (M: gmap Z (argmax Z)) (q: frac) 
       (bot: bot_gname) (subs: list sub_gname) : iProp Σ := 
-      ∃ (l:loc) (head: node_rep),
-      ⌜ #l = v ⌝
-      ∗
-      l ↦{#q} rep_to_node head
-      ∗
-      ⌜ node_key head = INT_MIN ⌝
-      ∗
-      skip_list_equiv MAX_HEIGHT head Smap q bot subs.
+      ∃ (head: node_rep),
+        p ↦□ rep_to_node head
+        ∗
+        ⌜ node_key head = INT_MIN ⌝
+        ∗
+        skip_list_equiv MAX_HEIGHT head M q bot subs.
 
     
-    Lemma skip_list_equiv_cons (head: node_rep) (lvl: Z) (Smap: gmap Z (argmax Z)) 
+    Lemma skip_list_equiv_cons (head: node_rep) (lvl: Z) (M: gmap Z (argmax Z)) 
       (q: frac) (bot: bot_gname) (top_sub: sub_gname) (bot_subs: list sub_gname) :
-      skip_list_equiv lvl head Smap q bot (top_sub :: bot_subs) ⊢ 
+      skip_list_equiv lvl head M q bot (top_sub :: bot_subs) ⊢ 
         ∃ (obot: option sub_gname),
           inv (levelN lvl) (lazy_list_inv lvl head bot top_sub obot)
           ∗
-          skip_list_equiv lvl head Smap q bot (top_sub :: bot_subs).
+          skip_list_equiv lvl head M q bot (top_sub :: bot_subs).
     Proof.
       destruct bot_subs as [|bot_sub bot_subs].
       + iIntros "Htop". iExists None.
-        iDestruct "Htop" as "(? & ? & #Hinv)".
-        iFrame "# ∗".
+        iDestruct "Htop" as "(%Hlvl & ? & #Hinv)".
+        subst; by iFrame "# ∗".
       + iIntros "Hlist". iExists (Some bot_sub).
         iDestruct "Hlist" as "(? & #Hinv & ?)".
         iFrame "# ∗".
     Qed.
 
-    Lemma skip_list_equiv_inv (lvl: Z) (head: node_rep) (Smap: gmap Z (argmax Z)) 
+    Lemma skip_list_equiv_inv (lvl: Z) (head: node_rep) (M: gmap Z (argmax Z)) 
       (q: frac) (bot: bot_gname) (subs: list sub_gname) :
-      skip_list_equiv lvl head Smap q bot subs ⊢
+      skip_list_equiv lvl head M q bot subs ⊢
         ∃ (sub: sub_gname),
           ⌜ last subs = Some sub ⌝
           ∗
-          is_bot_list 0 head Smap q bot sub
+          is_bot_list 0 head M q bot sub
           ∗
-          (is_bot_list 0 head Smap q bot sub -∗ skip_list_equiv lvl head Smap q bot subs).
+          (is_bot_list 0 head M q bot sub -∗ skip_list_equiv lvl head M q bot subs).
     Proof.
       iRevert (lvl).
       iInduction subs as [|top_sub subs] "IHsubs";
@@ -96,10 +94,10 @@ Module SkipListInv (Params: SKIP_LIST_PARAMS).
         iFrame.
     Qed.
 
-    Lemma skip_list_equiv_sep (lvl: Z) (head: node_rep) (Smap: gmap Z (argmax Z)) 
+    Lemma skip_list_equiv_sep (lvl: Z) (head: node_rep) (M: gmap Z (argmax Z)) 
       (q1 q2: frac) (bot: bot_gname) (subs: list sub_gname) :
-      skip_list_equiv lvl head Smap (q1 + q2) bot subs ⊢ 
-        skip_list_equiv lvl head Smap q1 bot subs ∗ skip_list_equiv lvl head Smap q2 bot subs.
+      skip_list_equiv lvl head M (q1 + q2) bot subs ⊢ 
+        skip_list_equiv lvl head M q1 bot subs ∗ skip_list_equiv lvl head M q2 bot subs.
     Proof.
       iRevert (lvl head).
       iInduction subs as [|top_sub bot_subs] "IHsubs"; 
@@ -115,10 +113,10 @@ Module SkipListInv (Params: SKIP_LIST_PARAMS).
         iSplitL "Hlist1"; by iFrame "# ∗".
     Qed.
 
-    Lemma skip_list_equiv_join (lvl: Z) (head: node_rep) (Smap1 Smap2: gmap Z (argmax Z)) 
+    Lemma skip_list_equiv_join (lvl: Z) (head: node_rep) (M1 M2: gmap Z (argmax Z)) 
       (q1 q2: frac) (bot: bot_gname) (subs: list sub_gname) :
-      skip_list_equiv lvl head Smap1 q1 bot subs ∗ skip_list_equiv lvl head Smap2 q2 bot subs ⊢ 
-        skip_list_equiv lvl head (merge op Smap1 Smap2) (q1 + q2) bot subs.
+      skip_list_equiv lvl head M1 q1 bot subs ∗ skip_list_equiv lvl head M2 q2 bot subs ⊢ 
+        skip_list_equiv lvl head (merge op M1 M2) (q1 + q2) bot subs.
     Proof.
       iRevert (lvl head).
       iInduction subs as [|top_sub bot_subs] "IHsubs"; 
@@ -137,37 +135,29 @@ Module SkipListInv (Params: SKIP_LIST_PARAMS).
         by iFrame "# ∗".
     Qed.
       
-    Lemma is_skip_list_sep (v: val) (Smap: gmap Z (argmax Z)) 
+    Lemma is_skip_list_sep (p: loc) (M: gmap Z (argmax Z)) 
       (q1 q2: frac) (bot: bot_gname) (subs: list sub_gname) :
-      is_skip_list v Smap (q1 + q2) bot subs ⊢ 
-        is_skip_list v Smap q1 bot subs ∗ is_skip_list v Smap q2 bot subs.
+      is_skip_list p M (q1 + q2) bot subs ⊢ 
+        is_skip_list p M q1 bot subs ∗ is_skip_list p M q2 bot subs.
     Proof.
       iIntros "Hlist".
-      iDestruct "Hlist" as (h head) "(%Hv & Hpt & %Hmin & Hlist)".
-
-      iDestruct "Hpt" as "(Hpt1 & Hpt2)".
+      iDestruct "Hlist" as (head) "(#Hpt & %Hmin & Hlist)".
       iDestruct (skip_list_equiv_sep with "Hlist") as "(Hlist1 & Hlist2)".
-
-      iSplitL "Hpt1 Hlist1"; iExists h, head; by iFrame.
+      iSplitL "Hlist1"; iExists head; by iFrame "# ∗".
     Qed.      
     
-    Lemma is_skip_list_join (v: val) (Smap1 Smap2: gmap Z (argmax Z))
+    Lemma is_skip_list_join (p: loc) (M1 M2: gmap Z (argmax Z))
       (q1 q2: frac) (bot: bot_gname) (subs: list sub_gname) :
-      is_skip_list v Smap1 q1 bot subs ∗ is_skip_list v Smap2 q2 bot subs ⊢ 
-        is_skip_list v (merge op Smap1 Smap2) (q1 + q2) bot subs.
+      is_skip_list p M1 q1 bot subs ∗ is_skip_list p M2 q2 bot subs ⊢ 
+        is_skip_list p (merge op M1 M2) (q1 + q2) bot subs.
     Proof.
       iIntros "(Hlist1 & Hlist2)".
-      iDestruct "Hlist1" as (h head) "(%Hv & Hpt1 & %Hmin & Hlist1)".
-      iDestruct "Hlist2" as (h' head') "(%Hv' & Hpt2 & _ & Hlist2)".
-
-      assert (h = h') as <- by congruence.
+      iDestruct "Hlist1" as (head) "(#Hpt1 & %Hmin & Hlist1)".
+      iDestruct "Hlist2" as (head') "(#Hpt2 & _ & Hlist2)".
       iDestruct (mapsto_agree with "Hpt1 Hpt2") as %<-%rep_to_node_inj.
-      iCombine "Hpt1 Hpt2" as "Hpt".
-
       iCombine "Hlist1 Hlist2" as "Hlist".
       rewrite skip_list_equiv_join.
-
-      iExists h, head. by iFrame.
+      iExists head; by iFrame "# ∗".
     Qed.
 
   End Proofs.
