jellyfish/spec/find.v
@@ -20,26 +20,26 @@ Module FindSpec (Params: SKIP_LIST_PARAMS).
   Section Proofs.
     Context `{!heapGS Σ, !skipGS Σ, !lockG Σ}.
     
-    Theorem find_bot_spec (key: Z) (head curr: node_rep) 
-      (Smap: gmap Z (argmax Z)) (bot: bot_gname) (sub: sub_gname) :
+    Theorem find_bot_spec (k: Z) (head curr: node_rep) 
+      (M: gmap Z (argmax Z)) (bot: bot_gname) (sub: sub_gname) :
       {{{ 
         inv (levelN 0) (lazy_list_inv 0 head bot sub None)
         ∗
-        own (s_frac bot) (◯F Smap)
+        own (s_frac bot) (◯F M)
         ∗
         (⌜ curr = head ⌝ ∨ own (s_auth sub) (◯ {[ curr ]}))
         ∗
-        ⌜ node_key curr < key < INT_MAX ⌝
+        ⌜ node_key curr < k < INT_MAX ⌝
       }}}
-        find (rep_to_node curr) #key #0
+        find (rep_to_node curr) #k #0
       {{{ pred succ, RET ((rep_to_node pred), (rep_to_node succ));
-        own (s_frac bot) (◯F Smap)
+        own (s_frac bot) (◯F M)
         ∗
-        ⌜ node_key pred < key ⌝
+        ⌜ node_key pred < k ⌝
         ∗
         (own (s_auth sub) (◯ {[ succ ]}) ∨ ⌜ succ = tail ⌝)
         ∗
-        ⌜ key ∈ dom Smap ↔ node_key succ = key ⌝
+        ⌜ k ∈ dom M ↔ node_key succ = k ⌝
       }}}.
     Proof.
       iIntros (Φ) "(#Hinv & Hown_frag & Hown_curr & Hrange) HΦ".
@@ -50,7 +50,7 @@ Module FindSpec (Params: SKIP_LIST_PARAMS).
       wp_lam. wp_pures.
 
       wp_bind (Load #(node_next curr +ₗ 0)).
-      iInv (levelN 0) as (S ? L) "(Hinv_sub & >Hown_frac)" "Hclose".
+      iInv (levelN 0) as (? S L) "(Hinv_sub & >Hown_frac)" "Hclose".
       iDestruct "Hinv_sub" as "(>%Hperm & >%Hsort & >%Hequiv & >Hown_auth & >Hown_toks & Hlist)".
       iDestruct (own_valid_2 with "Hown_frac Hown_frac_frag") 
         as %->%frac_auth_agree_L.
@@ -72,7 +72,7 @@ Module FindSpec (Params: SKIP_LIST_PARAMS).
         as (Ls&Lf&(Hcurr&Hsub)).
       { rewrite in_inv //. }
 
-      edestruct (node_rep_split_join Lf curr tail key) 
+      edestruct (node_rep_split_join Lf curr tail k) 
         as (pred&succ&L1&L2&?&?&Hpred_range&Hsucc_range&Hsplit_join); auto.
       {
         rewrite /= app_comm_cons Hcurr app_ass in Hsort.
@@ -80,7 +80,7 @@ Module FindSpec (Params: SKIP_LIST_PARAMS).
         simpl in *. by destruct Hsort as [_ ?].
       }
 
-      feed pose proof (node_rep_split_sep L Ls Lf L1 L2 head curr pred succ tail key) 
+      feed pose proof (node_rep_split_sep L Ls Lf L1 L2 head curr pred succ tail k) 
         as Htemp; auto.
       destruct Htemp as [Lm Hsplit_sep].
 
@@ -92,7 +92,7 @@ Module FindSpec (Params: SKIP_LIST_PARAMS).
         wp_load.
         iPoseProof ("Himp" with "Hpt") as "Hlist".
         iMod ("Hclose" with "[Hlist Hown_auth Hown_toks Hown_frac]") as "_".
-        { iNext; iExists S, Smap, L; by iFrame. }
+        { iNext; iExists M, S, L; by iFrame. }
 
         iModIntro. wp_load. 
         wp_let. wp_lam. wp_pures.
@@ -115,7 +115,7 @@ Module FindSpec (Params: SKIP_LIST_PARAMS).
         split; intros.
         * eapply (sorted_node_lt_cover_gap (Ls ++ L1) L2 pred); try lia.
           ++ by rewrite app_ass -Hsplit_join //= app_comm_cons -app_ass -Hcurr -app_comm_cons.
-          ++ assert (In key (map node_key (head :: L ++ [tail]))) as Hin.
+          ++ assert (In k (map node_key (head :: L ++ [tail]))) as Hin.
              { 
                right. 
                rewrite map_app in_app_iff -elem_of_list_In. 
@@ -167,7 +167,7 @@ Module FindSpec (Params: SKIP_LIST_PARAMS).
         wp_load.
         iPoseProof ("Himp" with "Hpt") as "Hlist".
         iMod ("Hclose" with "[Hlist Hown_auth Hown_toks Hown_frac]") as "_".
-        { iNext; iExists S, Smap, L; by iFrame. }
+        { iNext; iExists M, S, L; by iFrame. }
 
         iModIntro. wp_load. 
         wp_let. wp_lam. wp_pures.
@@ -211,18 +211,18 @@ Module FindSpec (Params: SKIP_LIST_PARAMS).
           iNext; iApply "HΦ".
     Qed.
     
-    Theorem find_sub_spec (key lvl: Z) (head curr: node_rep)
+    Theorem find_sub_spec (k lvl: Z) (head curr: node_rep)
       (bot: bot_gname) (sub: sub_gname) (obot: option sub_gname) :
       {{{ 
         inv (levelN lvl) (lazy_list_inv lvl head bot sub obot)
         ∗
         (⌜ curr = head ⌝ ∨ own (s_auth sub) (◯ {[ curr ]}))
         ∗
-        ⌜ node_key curr < key < INT_MAX ⌝
+        ⌜ node_key curr < k < INT_MAX ⌝
       }}}
-        find (rep_to_node curr) #key #lvl
+        find (rep_to_node curr) #k #lvl
       {{{ pred succ, RET ((rep_to_node pred), (rep_to_node succ));
-        ⌜ node_key pred < key ≤ node_key succ ⌝
+        ⌜ node_key pred < k ≤ node_key succ ⌝
         ∗
         (⌜ pred = head ⌝ ∨ own (s_auth sub) (◯ {[ pred ]}))
         ∗
@@ -242,7 +242,7 @@ Module FindSpec (Params: SKIP_LIST_PARAMS).
       wp_lam. wp_pures.
 
       wp_bind (Load #(node_next curr +ₗ lvl)).
-      iInv (levelN lvl) as (S Smap L) "(Hinv_sub & Hmatch)" "Hclose".
+      iInv (levelN lvl) as (M S L) "(Hinv_sub & Hmatch)" "Hclose".
       iDestruct "Hinv_sub" as "(>%Hperm & >%Hsort & >%Hequiv & >Hown_auth & >Hown_toks & Hlist)".
 
       iMod (own_update with "Hown_auth") as "[Hown_auth Hown_frag]".
@@ -265,7 +265,7 @@ Module FindSpec (Params: SKIP_LIST_PARAMS).
       wp_load.
       iPoseProof ("Himp" with "Hpt") as "Hlist".
       iMod ("Hclose" with "[Hmatch Hlist Hown_auth Hown_toks]") as "_".
-      { iNext; iExists S, Smap, L; by iFrame. }
+      { iNext; iExists M, S, L; by iFrame. }
 
       iModIntro. wp_load.
       wp_let. wp_lam. wp_pures.
@@ -297,18 +297,18 @@ Module FindSpec (Params: SKIP_LIST_PARAMS).
         iNext; iApply "HΦ".
     Qed.
 
-    Theorem findLock_spec (key lvl: Z) (head curr: node_rep)
+    Theorem findLock_spec (k lvl: Z) (head curr: node_rep)
       (bot: bot_gname) (sub: sub_gname) (obot: option sub_gname) :
       {{{ 
         inv (levelN lvl) (lazy_list_inv lvl head bot sub obot)
         ∗
         (⌜ curr = head ⌝ ∨ own (s_auth sub) (◯ {[ curr ]}))
         ∗
-        ⌜ node_key curr < key < INT_MAX ⌝
+        ⌜ node_key curr < k < INT_MAX ⌝
       }}}
-        findLock (rep_to_node curr) #key #lvl
+        findLock (rep_to_node curr) #k #lvl
       {{{ pred succ, RET ((rep_to_node pred), (rep_to_node succ));
-        ⌜ node_key pred < key ≤ node_key succ ⌝
+        ⌜ node_key pred < k ≤ node_key succ ⌝
         ∗
         (⌜ pred = head ⌝ ∨ own (s_auth sub) (◯ {[ pred ]}))
         ∗
@@ -323,7 +323,7 @@ Module FindSpec (Params: SKIP_LIST_PARAMS).
           ∗
           s ↦□ rep_to_node succ
           ∗
-          locked_val obot succ
+          locked_val obot s
           ∗
           locked γ
       }}}.
@@ -336,7 +336,7 @@ Module FindSpec (Params: SKIP_LIST_PARAMS).
       wp_lam. wp_let. wp_let.
       wp_apply (find_sub_spec with "[Hown_curr]").
       { by iFrame "#". }
-      iIntros (pred succ) "(%Hrange' & #Hown_pred & #Hown_succ & Hlock)".
+      iIntros (pred succ'') "(%Hrange' & #Hown_pred & _ & Hlock)".
       iDestruct "Hlock" as (γ l) "(#Hl & #Hlock)".
       wp_pures. wp_lam. wp_pures.
 
@@ -344,60 +344,64 @@ Module FindSpec (Params: SKIP_LIST_PARAMS).
       wp_bind (acquire _).
       iApply (acquire_spec with "Hlock").
       iNext; iIntros "(Hlocked & Hin_lock)".
-      iDestruct "Hin_lock" as (s succ') "(Hnext & #Hs & Hval)".
+      iDestruct "Hin_lock" as (s) "(Hnext & Hval)".
 
       wp_pures. wp_lam. wp_pures.
       wp_bind (Load #(node_next pred +ₗ lvl)).
-      iInv (levelN lvl) as (S Smap L) "(Hinv_sub & Hmatch)" "Hclose".
+      iInv (levelN lvl) as (M S L) "(Hinv_sub & Hmatch)" "Hclose".
       iDestruct "Hinv_sub" as "(>%Hperm & >%Hsort & >%Hequiv & >Hown_auth & >Hown_toks & Hlist)".
 
-      iAssert (⌜ pred = head ∨ In pred L ⌝ ∗ ⌜ In succ L ∨ succ = tail ⌝)%I
-        with "[Hown_auth Hown_pred Hown_succ]" as "(%Hpred_range & %Hsucc_range)".
+      iMod (own_update with "Hown_auth") as "[Hown_auth Hown_frag]".
+      { by apply auth_update_alloc, (gset_local_update S _ S). }
+
+      iAssert ⌜ pred = head ∨ In pred L ⌝%I
+        with "[Hown_auth Hown_pred]" as %Hpred_range.
       {
-        iSplit.
-        + iDestruct "Hown_pred" as "[Heq|Hown]"; first by iLeft.
-          iDestruct (own_valid_2 with "Hown_auth Hown") 
-            as %[Hvalid%gset_included]%auth_both_valid_discrete.
-          iPureIntro; right.
-          rewrite -elem_of_list_In Hperm elem_of_elements. 
-          set_solver.
-        + iDestruct "Hown_succ" as "[Hown|Heq]"; last by iRight.
-          iDestruct (own_valid_2 with "Hown_auth Hown") 
-            as %[Hvalid%gset_included]%auth_both_valid_discrete.
-          iPureIntro; left.
-          rewrite -elem_of_list_In Hperm elem_of_elements.
-          set_solver.
+        iDestruct "Hown_pred" as "[Heq|Hown]"; first by iLeft.
+        iDestruct (own_valid_2 with "Hown_auth Hown") 
+          as %[Hvalid%gset_included]%auth_both_valid_discrete.
+        iPureIntro; right.
+        rewrite -elem_of_list_In Hperm elem_of_elements. 
+        set_solver.
       }
 
       rewrite list_equiv_invert; last done.
-      iDestruct "Hlist" as (γ' l' s' succ'') "(>%Hsucc''_in_L & >Hpt & >#Hs' & _ & _ & Himp)".
-      iDestruct (mapsto_agree with "Hnext Hpt") as %Hs.
+      iDestruct "Hlist" as (γ' l' s' succ) "(>%Hsucc_range & >Hpt & >#Hs' & _ & _ & Himp)".
+      rewrite -elem_of_list_In Hperm elem_of_elements in Hsucc_range.
+      iDestruct (mapsto_agree with "Hpt Hnext") as %Hs.
       inversion Hs; subst.
-      iDestruct (mapsto_agree with "Hs Hs'") as %<-%rep_to_node_inj.
+
+      iAssert (own (s_auth sub) (◯ {[succ]}) ∨ ⌜ succ = tail ⌝)%I
+        with "[Hown_frag]" as "#Hown_succ".
+      {
+        destruct Hsucc_range as [Hin|Heq]; last by iRight.
+        assert (S = S ⋅ {[ succ ]}) as -> by set_solver.
+        iDestruct "Hown_frag" as "(? & ?)"; iLeft; iFrame.
+      }
 
       wp_load.
       iPoseProof ("Himp" with "Hpt") as "Hlist".
       iMod ("Hclose" with "[Hmatch Hlist Hown_auth Hown_toks]") as "_".
-      { iNext; iExists S, Smap, L; by iFrame. }
+      { iNext; iExists M, S, L; by iFrame. }
 
       iModIntro. wp_load.
-      wp_let. wp_lam. wp_pures. wp_lam. wp_pures.
-      case_bool_decide as Heq; wp_if.
-      + iModIntro; iApply "HΦ".
-        iFrame "# ∗".
-        iSplit; first done. iExists γ, l, s'.
-
-        assert (succ = succ') as <-; last by iFrame "# ∗".
-        apply (sorted_node_key_unique (L ++ [tail])).
-        - apply node_rep_sorted_app in Hsort; by destruct Hsort.
-        - by rewrite in_inv_rev.
-        - by rewrite in_inv_rev. 
-        - congruence.
+      wp_let. wp_lam. wp_pures.
+      case_bool_decide as Hle; wp_if.
+      + wp_pures; iApply "HΦ".
+        iModIntro; iFrame "#".
+        iSplit; first by (iPureIntro; lia).
+        iExists γ, l, s. iFrame "# ∗".
       + wp_apply (release_spec with "[Hnext Hval Hlocked]").
-        { iFrame "# ∗"; iExists s', succ'; iFrame "# ∗". }
-        iIntros. wp_pures.
-        iApply ("IH" with "HΦ Hown_pred"). 
-        iPureIntro; lia.
+        { iFrame "# ∗"; iExists s; iFrame. }
+        iIntros "_". wp_pures.
+
+        iApply ("IH" with "HΦ [] [%]").
+        {
+          iRight.
+          iDestruct "Hown_succ" as "[Hown|%Htail]"; first done.
+          rewrite Htail /node_key/tail/= in Hle; lia.
+        }
+        { lia. }
     Qed.
 
   End Proofs.
