jellyfish/spec/link.v
@@ -19,190 +19,6 @@ Module LinkSpec (Params: SKIP_LIST_PARAMS).
   Section Proofs.
     Context `{!heapGS Σ, !skipGS Σ, !lockG Σ}.
 
-    Theorem createAndLink_spec (key v ts h: Z) (head pred succ: node_rep) 
-      (Smap: gmap Z (argmax Z)) (q: frac)
-      (sub: sub_gname) (bot: bot_gname) (s: loc) :
-      INT_MIN < key < INT_MAX →
-      {{{ 
-        is_bot_list 0 head Smap q bot sub
-        ∗
-        (⌜ pred = head ⌝ ∨ own (s_auth sub) (◯ {[ pred ]}))
-        ∗
-        ⌜ node_key pred < key < node_key succ ⌝
-        ∗
-        node_next pred ↦{#1 / 2} #s
-        ∗
-        s ↦□ rep_to_node succ
-        ∗
-        locked_val None succ
-        ∗
-        ⌜ 0 ≤ h ⌝ 
-      }}}
-        createAndLink (rep_to_node pred) #key #v #ts #h
-      {{{ (n: loc) (new: node_rep), RET #n;
-        is_bot_list 0 head (Smap ⋅ {[ key := prodZ {[ v ]} ts ]}) q bot sub
-        ∗
-        own (s_auth sub) (◯ {[ new ]})
-        ∗ 
-        own (s_toks sub) (GSet {[ node_key new ]})
-        ∗ 
-        ⌜ node_key new = key ⌝
-        ∗ 
-        node_next pred ↦{#1 / 2} #n
-        ∗
-        n ↦□ rep_to_node new
-        ∗
-        node_val new ↦{#1 / 2} rep_to_val (v, ts, dummy_null)%core
-        ∗
-        (node_next new +ₗ 1) ↦∗ replicate (Z.to_nat h) #()
-        ∗
-        (node_locks new +ₗ 1) ↦∗ replicate (Z.to_nat h) #()
-      }}}.
-    Proof.
-      iIntros (Hkey_range Φ) "(Hbot & #Hown_pred & %Hrange & Hpt & #Hs & Hval & %Hlvl) HΦ".
-      iDestruct "Hbot" as "(Hown_frag & #Hinv)".
-
-      wp_lam. wp_pures. 
-      wp_lam. wp_pures.
-      wp_load. wp_let. 
-
-      wp_alloc next as "Hnext"; first lia. wp_let.
-      wp_alloc locks as "Hlocks"; first lia. wp_let.
-      assert (Z.to_nat (h + 1) = S (Z.to_nat h)) as -> by lia.
-      rewrite replicate_S ?array_cons.
-      iDestruct "Hnext" as "(Hn & Hnext)".
-      iDestruct "Hlocks" as "(Hlocks' & Hlocks)".
-
-      set (val := (v, ts, dummy_null)).
-      wp_alloc vpt as "Hvpt". wp_let.
-      iDestruct "Hvpt" as "(Hvpt & Hvpt')".
-      rewrite (fold_rep_to_val val).
-
-      set (new := (key, vpt, next, @None loc, #(), locks)).
-      wp_alloc node as "Hnode". wp_let.
-      iMod (mapsto_persist with "Hnode") as "#Hnode".
-      rewrite (fold_rep_to_node new).
-
-      wp_store; iDestruct "Hn" as "(Hn & Hn')".
-
-      wp_apply (newlock_spec (in_lock 0 None new) with "[Hn' Hval]").
-      { iExists s, succ; rewrite loc_add_0; iFrame "# ∗". }
-      iIntros (l γ) "#Hlock".
-      wp_store; iMod (mapsto_persist with "Hlocks'") as "#Hl".
-
-      wp_bind (Store _ _).
-      iInv (levelN 0) as (S' Smap' L) "(Hinv_sub & >Hown_frac)" "Hclose".
-      iDestruct "Hinv_sub" as "(>%Hperm & >%Hsort & >%Hequiv & >Hown_auth & >Hown_toks & Hlist)".
-
-      iAssert ⌜ pred = head ∨ In pred L ⌝%I
-        with "[Hown_auth Hown_pred]" as %Hpred_range.
-      {
-        iDestruct "Hown_pred" as "[Heq|Hown]"; first by iLeft.
-        iDestruct (own_valid_2 with "Hown_auth Hown") 
-          as %[Hvalid%gset_included]%auth_both_valid_discrete.
-        iPureIntro; right. 
-        rewrite -elem_of_list_In Hperm elem_of_elements.
-        set_solver.
-      }
-
-      rewrite (list_equiv_join 0 None s head pred succ); auto.
-      rewrite loc_add_0. 
-      iDestruct ("Hlist" with "[Hpt]") as "Hlist".
-      { iNext; iFrame "# ∗". }
-      iDestruct "Hlist" as (L1 L2) "(>%Hsplit & Hpt & Hlist)".
-
-      assert (key ∉ dom Smap') as Hnin'.
-      {
-        intros Hfalse.
-        rewrite -elem_of_elements Hequiv elem_of_list_In -Hperm in_map_iff in Hfalse.
-        destruct Hfalse as [x [Hkey Hin]].
-        
-        apply (sorted_node_lt_nin L1 L2 pred succ x).
-        { rewrite -Hsplit //. }
-        { rewrite Hkey; lia. }
-        rewrite -Hsplit. apply in_or_app; right. apply in_or_app; by left.
-      }
-
-      assert (Smap' !! key = None) as Hnone.
-      { rewrite -not_elem_of_dom //. }
-
-      rewrite (list_equiv_insert 0 None s node head pred new succ L val γ l); first last.
-      { done. }
-      { done. }
-      { done. }
-      { assert (node_key new = key) as -> by auto; lia. }
-      { rewrite /node_key/=; lia. }
-
-      rewrite ?loc_add_0.
-      iDestruct ("Hlist" with "[Hpt Hn Hvpt']") as "Hlist".
-      { iNext; iFrame "# ∗". }
-      iDestruct "Hlist" as (L') "(Hpt & >%Hsort' & >%Hperm' & Himp)".
-
-      iDestruct (own_valid_2 with "Hown_frac Hown_frag") 
-        as %HsubSmap%frac_auth_included_total.
-
-      iMod (own_update with "Hown_auth") as "[Hown_auth Hown_auth_frag]".
-      { apply auth_update_alloc, (gset_local_update_union _ _ {[ new ]}). }
-      assert (ε ∪ {[ new ]} = {[ new ]}) as -> by set_solver.
-
-      iMod (own_update_2 with "Hown_frac Hown_frag") as "[Hown_frac Hown_frac_frag]".
-      { apply frac_auth_update, (alloc_local_update _ _ key (prodZ {[ v ]} ts)); done. }
-
-      rewrite (gset_union_diff key); first last.
-      { done. }
-      { rewrite Zlt_range_spec; lia. }
-      rewrite -gset_disj_union; last set_solver.
-      iDestruct "Hown_toks" as "(Hown_toks & Hown_tok)".
-
-      wp_store.
-      iDestruct "Hpt" as "(Hpt & Hpt_dup)".
-      iPoseProof ("Himp" with "Hpt_dup") as "Hlist".
-      iMod ("Hclose" with "[Hlist Hown_auth Hown_toks Hown_frac]") as "_".
-      {
-        iNext; iExists (S' ∪ {[ new ]}), (<[ key := prodZ {[ v ]} ts ]>Smap'), L'.
-        pose proof (dom_insert Smap' key (prodZ {[v]} ts)) as Hdom.
-        rewrite leibniz_equiv_iff comm_L in Hdom.
-        rewrite Hdom.
-        iFrame. iPureIntro.
-
-        split; first last. 
-        { split; first done. by apply key_equiv_insert_nin. }
-        
-        apply NoDup_Permutation.
-        { 
-          apply node_rep_sorted_app in Hsort'; destruct Hsort' as [_ Hsort']. 
-          apply node_rep_sorted_app in Hsort'; destruct Hsort' as [Hsort' _].
-          by apply sorted_node_lt_no_dup.
-        } 
-        { apply NoDup_elements. }
-
-        simpl in Hperm'; apply Permutation_cons_inv in Hperm'.
-        intros x; split.
-        + rewrite elem_of_elements Hperm' elem_of_list_In.
-          intros Hin. destruct Hin as [Heq|Hin].
-          - set_solver.
-          - apply elem_of_union_l. 
-            by rewrite -elem_of_elements -Hperm elem_of_list_In.
-        + rewrite elem_of_elements Hperm'. 
-          intros Hin. apply elem_of_union in Hin as [Hin|Heq].
-          - rewrite elem_of_list_In. right.
-            by rewrite -elem_of_list_In Hperm elem_of_elements.
-          - set_solver.
-      }
-
-      iModIntro; wp_pures. 
-      iModIntro; iApply "HΦ".
-
-      rewrite insert_singleton_op; last first.
-      {
-        rewrite lookup_included in HsubSmap.
-        destruct (HsubSmap key) as [z Heq%leibniz_equiv_iff].
-        rewrite Hnone comm op_None in Heq.
-        by destruct Heq.
-      }
-      rewrite comm_L. by iFrame "# ∗". 
-    Qed.
-
     Theorem link_spec (lvl: Z) (head pred new succ: node_rep) 
       (bot: bot_gname) (top_sub bot_sub: sub_gname) 
       (v: val_rep) (s n: loc) :
@@ -237,20 +53,20 @@ Module LinkSpec (Params: SKIP_LIST_PARAMS).
     Proof.
       iIntros (Hkey_range Φ) "(#Hinv & #Hown_pred & %Hrange & Hpt & #Hs & Hnode & #Hn & Hnext & Hl) HΦ".
 
-      wp_lam. wp_pures. wp_lam. wp_pures.
-      wp_load. wp_let. 
-      wp_load. wp_lam. wp_pures. 
-      wp_load. wp_lam. wp_pures.
-      
+      wp_lam. wp_pures.
+      wp_load. wp_let.
+      wp_lam. wp_pures. wp_load.
+      wp_lam. wp_pures.       
       wp_store; iDestruct "Hnext" as "(Hnext & Hnext')".
 
       wp_apply (newlock_spec (in_lock lvl (Some bot_sub) new) with "[Hnext']").
-      { iExists s, succ; iFrame "# ∗". }
+      { iExists s; iFrame. }
       iIntros (l γ) "#Hlock".
+      wp_lam. wp_pures.
       wp_store; iMod (mapsto_persist with "Hl") as "#Hl".
       
-      wp_pures.
-      iInv (levelN lvl) as (S' Smap' L) "(Hinv_sub & _)" "Hclose".
+      wp_lam. wp_pures.
+      iInv (levelN lvl) as (M' S' L) "(Hinv_sub & _)" "Hclose".
       iDestruct "Hinv_sub" as "(>%Hperm & >%Hsort & >%Hequiv & >Hown_auth & >Hown_toks & Hlist)".
 
       iAssert ⌜ pred = head ∨ In pred L ⌝%I
@@ -269,7 +85,7 @@ Module LinkSpec (Params: SKIP_LIST_PARAMS).
       { iNext; iFrame "# ∗". }
       iDestruct "Hlist" as (L1 L2) "(>%Hsplit & Hpt & Hlist)".
 
-      assert (node_key new ∉ dom Smap') as Hnin'.
+      assert (node_key new ∉ dom M') as Hnin'.
       {
         intros Hfalse.
         rewrite -elem_of_elements Hequiv elem_of_list_In -Hperm in_map_iff in Hfalse.
@@ -281,7 +97,7 @@ Module LinkSpec (Params: SKIP_LIST_PARAMS).
         rewrite -Hsplit. apply in_or_app; right. apply in_or_app; by left.
       }
 
-      assert (Smap' !! node_key new = None) as Hnone.
+      assert (M' !! node_key new = None) as Hnone.
       { rewrite -not_elem_of_dom //. }
 
       rewrite (list_equiv_insert lvl (Some bot_sub) s n head pred new succ L v γ l); first last.
@@ -310,8 +126,8 @@ Module LinkSpec (Params: SKIP_LIST_PARAMS).
       iPoseProof ("Himp" with "Hpt_dup") as "Hlist".
       iMod ("Hclose" with "[Hlist Hown_auth Hown_toks]") as "_".
       {
-        iNext; iExists (S' ∪ {[ new ]}), (<[ node_key new := prodZ {[ val_v v ]} (val_ts v) ]>Smap'), L'.
-        pose proof (dom_insert Smap' (node_key new) (prodZ {[ val_v v ]} (val_ts v))) as Hdom.
+        iNext; iExists (<[ node_key new := prodZ {[ val_v v ]} (val_ts v) ]>M'), (S' ∪ {[ new ]}), L'.
+        pose proof (dom_insert M' (node_key new) (prodZ {[ val_v v ]} (val_ts v))) as Hdom.
         rewrite leibniz_equiv_iff comm_L in Hdom.
         rewrite Hdom.
         iFrame. iPureIntro.
@@ -343,6 +159,195 @@ Module LinkSpec (Params: SKIP_LIST_PARAMS).
 
       iModIntro. iApply "HΦ". 
       iFrame "# ∗". 
+    Qed.
+
+    Theorem createAndLink_spec (k v t h: Z) (head pred succ: node_rep) 
+      (M: gmap Z (argmax Z)) (q: frac)
+      (sub: sub_gname) (bot: bot_gname) (s: loc) :
+      INT_MIN < k < INT_MAX →
+      {{{ 
+        inv (levelN 0) (lazy_list_inv 0 head bot sub None)
+        ∗
+        own (s_frac bot) (◯F{q} M)
+        ∗
+        (⌜ pred = head ⌝ ∨ own (s_auth sub) (◯ {[ pred ]}))
+        ∗
+        ⌜ node_key pred < k < node_key succ ⌝
+        ∗
+        node_next pred ↦{#1 / 2} #s
+        ∗
+        s ↦□ rep_to_node succ
+        ∗
+        locked_val None s
+        ∗
+        ⌜ 0 ≤ h ⌝ 
+      }}}
+        createAndLink (rep_to_node pred) #k #v #t #h
+      {{{ (n: loc) (new: node_rep), RET #n;
+        own (s_frac bot) (◯F{q} (M ⋅ {[ k := prodZ {[ v ]} t ]}))
+        ∗
+        own (s_auth sub) (◯ {[ new ]})
+        ∗ 
+        own (s_toks sub) (GSet {[ node_key new ]})
+        ∗ 
+        ⌜ node_key new = k ⌝
+        ∗ 
+        node_next pred ↦{#1 / 2} #n
+        ∗
+        n ↦□ rep_to_node new
+        ∗
+        node_val new ↦{#1 / 2} rep_to_val (v, t, dummy_null)%core
+        ∗
+        (node_next new +ₗ 1) ↦∗ replicate (Z.to_nat h) #()
+        ∗
+        (node_locks new +ₗ 1) ↦∗ replicate (Z.to_nat h) #()
+      }}}.
+    Proof.
+      iIntros (Hkey_range Φ) "(#Hinv & Hown_frag & #Hown_pred & %Hrange & Hpt & #Hs & Hval & %Hlvl) HΦ".
+      wp_lam. wp_pures.
+      
+      wp_alloc next as "Hnext"; first lia. wp_let.
+      wp_alloc locks as "Hlocks"; first lia. wp_let.
+      assert (Z.to_nat (h + 1) = S (Z.to_nat h)) as -> by lia.
+      rewrite replicate_S ?array_cons.
+      iDestruct "Hnext" as "(Hn & Hnext)".
+      iDestruct "Hlocks" as "(Hlocks' & Hlocks)".
+
+      set (val := (v, t, dummy_null)).
+      wp_alloc vpt as "Hvpt". wp_let.
+      iDestruct "Hvpt" as "(Hvpt & Hvpt')".
+      rewrite (fold_rep_to_val val).
+
+      set (new := (k, vpt, next, @None loc, #(), locks)).
+      wp_alloc node as "Hnode". wp_let.
+      iMod (mapsto_persist with "Hnode") as "#Hnode".
+      rewrite (fold_rep_to_node new).
+
+      wp_lam. wp_let. wp_let.
+      wp_load. wp_let.
+      wp_lam; wp_pures; rewrite loc_add_0.
+      wp_load.
+      wp_lam; wp_pures; rewrite loc_add_0.
+      wp_store; iDestruct "Hn" as "(Hn & Hn')".
+
+      wp_apply (newlock_spec (in_lock 0 None new) with "[Hn' Hval]").
+      { iExists s; rewrite loc_add_0; iFrame. }
+      iIntros (l γ) "#Hlock".
+      wp_lam; wp_pures; rewrite loc_add_0.
+      wp_store; iMod (mapsto_persist with "Hlocks'") as "#Hl".
+
+      wp_lam; wp_pures; rewrite loc_add_0.
+      wp_bind (Store _ _).
+      iInv (levelN 0) as (M' S' L) "(Hinv_sub & >Hown_frac)" "Hclose".
+      iDestruct "Hinv_sub" as "(>%Hperm & >%Hsort & >%Hequiv & >Hown_auth & >Hown_toks & Hlist)".
+
+      iAssert ⌜ pred = head ∨ In pred L ⌝%I
+        with "[Hown_auth Hown_pred]" as %Hpred_range.
+      {
+        iDestruct "Hown_pred" as "[Heq|Hown]"; first by iLeft.
+        iDestruct (own_valid_2 with "Hown_auth Hown") 
+          as %[Hvalid%gset_included]%auth_both_valid_discrete.
+        iPureIntro; right. 
+        rewrite -elem_of_list_In Hperm elem_of_elements.
+        set_solver.
+      }
+
+      rewrite (list_equiv_join 0 None s head pred succ); auto.
+      rewrite loc_add_0. 
+      iDestruct ("Hlist" with "[Hpt]") as "Hlist".
+      { iNext; iFrame "# ∗". }
+      iDestruct "Hlist" as (L1 L2) "(>%Hsplit & Hpt & Hlist)".
+
+      assert (k ∉ dom M') as Hnin'.
+      {
+        intros Hfalse.
+        rewrite -elem_of_elements Hequiv elem_of_list_In -Hperm in_map_iff in Hfalse.
+        destruct Hfalse as [x [Hkey Hin]].
+        
+        apply (sorted_node_lt_nin L1 L2 pred succ x).
+        { rewrite -Hsplit //. }
+        { rewrite Hkey; lia. }
+        rewrite -Hsplit. apply in_or_app; right. apply in_or_app; by left.
+      }
+
+      assert (M' !! k = None) as Hnone.
+      { rewrite -not_elem_of_dom //. }
+
+      rewrite (list_equiv_insert 0 None s node head pred new succ L val γ l); first last.
+      { done. }
+      { done. }
+      { done. }
+      { assert (node_key new = k) as -> by auto; lia. }
+      { rewrite /node_key/=; lia. }
+
+      rewrite ?loc_add_0.
+      iDestruct ("Hlist" with "[Hpt Hn Hvpt']") as "Hlist".
+      { iNext; iFrame "# ∗". }
+      iDestruct "Hlist" as (L') "(Hpt & >%Hsort' & >%Hperm' & Himp)".
+
+      iDestruct (own_valid_2 with "Hown_frac Hown_frag") 
+        as %HsubM%frac_auth_included_total.
+
+      iMod (own_update with "Hown_auth") as "[Hown_auth Hown_auth_frag]".
+      { apply auth_update_alloc, (gset_local_update_union _ _ {[ new ]}). }
+      assert (ε ∪ {[ new ]} = {[ new ]}) as -> by set_solver.
+
+      iMod (own_update_2 with "Hown_frac Hown_frag") as "[Hown_frac Hown_frac_frag]".
+      { apply frac_auth_update, (alloc_local_update _ _ k (prodZ {[ v ]} t)); done. }
+
+      rewrite (gset_union_diff k); first last.
+      { done. }
+      { rewrite Zlt_range_spec; lia. }
+      rewrite -gset_disj_union; last set_solver.
+      iDestruct "Hown_toks" as "(Hown_toks & Hown_tok)".
+
+      wp_store.
+      iDestruct "Hpt" as "(Hpt & Hpt_dup)".
+      iPoseProof ("Himp" with "Hpt_dup") as "Hlist".
+      iMod ("Hclose" with "[Hlist Hown_auth Hown_toks Hown_frac]") as "_".
+      {
+        iNext; iExists (<[ k := prodZ {[ v ]} t ]>M'), (S' ∪ {[ new ]}), L'.
+        pose proof (dom_insert M' k (prodZ {[v]} t)) as Hdom.
+        rewrite leibniz_equiv_iff comm_L in Hdom.
+        rewrite Hdom.
+        iFrame. iPureIntro.
+
+        split; first last. 
+        { split; first done. by apply key_equiv_insert_nin. }
+        
+        apply NoDup_Permutation.
+        { 
+          apply node_rep_sorted_app in Hsort'; destruct Hsort' as [_ Hsort']. 
+          apply node_rep_sorted_app in Hsort'; destruct Hsort' as [Hsort' _].
+          by apply sorted_node_lt_no_dup.
+        } 
+        { apply NoDup_elements. }
+
+        simpl in Hperm'; apply Permutation_cons_inv in Hperm'.
+        intros x; split.
+        + rewrite elem_of_elements Hperm' elem_of_list_In.
+          intros Hin. destruct Hin as [Heq|Hin].
+          - set_solver.
+          - apply elem_of_union_l. 
+            by rewrite -elem_of_elements -Hperm elem_of_list_In.
+        + rewrite elem_of_elements Hperm'. 
+          intros Hin. apply elem_of_union in Hin as [Hin|Heq].
+          - rewrite elem_of_list_In. right.
+            by rewrite -elem_of_list_In Hperm elem_of_elements.
+          - set_solver.
+      }
+
+      iModIntro; wp_pures. 
+      iModIntro; iApply "HΦ".
+
+      rewrite insert_singleton_op; last first.
+      {
+        rewrite lookup_included in HsubM.
+        destruct (HsubM k) as [z Heq%leibniz_equiv_iff].
+        rewrite Hnone comm op_None in Heq.
+        by destruct Heq.
+      }
+      rewrite comm_L. by iFrame "# ∗". 
     Qed.
 
   End Proofs.
